Added inl case to preservation proof

bigstep.v
@@ -5,8 +5,10 @@ Require Import meta_term.
 Require Import meta_subst.
 Require Import comp_expr.
 Require Import unification.
+Require Import Coq.Program.Equality.
 
 Reserved Notation "E ⇓ V" (at level 90).
+
 
 Inductive val : closure -> Prop :=
  | fn_val : forall γ δ δ' (θ:msubst γ ∅) (y:δ↪δ') E ρ,
@@ -14,6 +16,19 @@ Inductive val : closure -> Prop :=
  | mlam_val : forall γ γ' δ θ (X:γ↪γ') E (ρ:env δ),
       env_val ρ -> val ((mlam X E)[θ;;ρ])
  | meta_term_val : forall C, val (meta_term_closure C)
+ | tt_val : forall γ δ (θ:msubst γ ∅) (ρ:env δ),
+      env_val ρ -> val (tt[θ;;ρ])
+ | inl_val : forall γ δ (θ:msubst γ ∅) (ρ:env δ) E,
+      env_val ρ -> val (E[θ;;ρ]) -> val ((inl E)[θ;;ρ])
+ | inr_val : forall γ δ (θ:msubst γ ∅) (ρ:env δ) E,
+      env_val ρ -> val (E[θ;;ρ]) -> val ((inr E)[θ;;ρ])
+ | pair_val : forall γ δ (θ:msubst γ ∅) (ρ:env δ) E1 E2,
+      env_val ρ -> val (E1[θ;;ρ]) -> val (E2[θ;;ρ])
+      -> val ((pair E1 E2)[θ;;ρ]) 
+ | fold_val : forall γ δ (θ:msubst γ ∅) (ρ:env δ) E,
+      env_val ρ -> val (E[θ;;ρ]) -> val ((fold E)[θ;;ρ])
+ | pack_val : forall γ δ (θ:msubst γ ∅) (ρ:env δ) E C,
+      env_val ρ -> val (E[θ;;ρ]) -> val ((pack C E)[θ;;ρ])
 with env_val : forall {δ}, env δ -> Prop :=
  | env_val_nil : env_val ·
  | env_val_cons : forall γ (ρ:env γ) γ' (y:γ↪γ') V,
@@ -63,8 +78,21 @@ Inductive eval : closure -> closure -> Prop :=
  | ev_rec : forall δ θ γ ρ γ' (f:γ↪γ') (E:checked_exp δ γ') V,
        E [ θ ;; ρ ,, (f, (rec f E)[θ;;ρ]) ] ⇓ V
     -> rec f E [θ ;; ρ] ⇓ V
+ | ev_inl : forall δ (θ:msubst δ ∅) γ (ρ:env γ) E
+            δ' (θ':msubst δ' ∅) γ' (ρ':env γ') V,
+            E[θ;;ρ] ⇓ V[θ';;ρ']
+         -> (inl E)[θ;;ρ] ⇓ (inl V)[θ';;ρ']
 where "E1 ⇓ V1" := (eval E1 V1).
 
+Hint Constructors val.
+
+Lemma val_env_val δ γ (θ:msubst δ ∅) (ρ:env γ) V
+ (H:val (V [θ;;ρ])) : env_val ρ.
+inversion H; subst; simpl_existTs; subst; eauto.
+Qed.
+Hint Resolve val_env_val.
+
 Theorem eval_val L V : L ⇓ V -> val V.
-induction 1; assumption.
+induction 1; try assumption;
+econstructor; eauto.
 Qed.
